ar/theories/Dec.v
@@ -1,110 +1,26 @@
 Require Import Ascii.
 
-Class Decidable (P : Prop) := {
-	is_dec : {P} + {~ P};
-}.
+Inductive Decidable (P : Prop) : Prop :=
+| dec_true : P -> Decidable P
+| dec_false : ~ P -> Decidable P.
 
-Definition dec (P : Prop) {Hd : Decidable P} : bool :=
-	match (@is_dec P Hd) with
-		| left _ => true
-		| right _ => false
-	end.
+Inductive pbool : Prop :=
+| ptrue
+| pfalse.
 
-Notation "# P" := (dec P) (at level 70).
+Definition compute_dec (P : Prop) {d : Decidable P} :=
+match d with
+| dec_true _ _ => ptrue
+| dec_false _ _ => pfalse
+end.
 
-Lemma dec_true : forall (P : Prop) `{Decidable P}, ((# P) = true) <-> P.
-split; intros.
-+ case_eq is_dec; intros; trivial.
-	unfold dec in H0.
-	rewrite H1 in H0.
-	discriminate H0.
-+ case_eq is_dec; intros.
-	- unfold dec.
-		now rewrite H1.
-	- now absurd (P).
+Lemma DecidableBoolEq (a b : bool) : (Decidable (a = b)).
+Proof.
+destruct a; destruct b; try (now left); now right.
 Qed.
 
-Lemma dec_false : forall (P : Prop) `{Decidable P}, ((# P) = false) <-> ~P.
-split; intros.
-+ case_eq is_dec; intros; trivial.
-	unfold dec in H0.
-	rewrite H1 in H0.
-	discriminate H0.
-+ case_eq is_dec; intros.
-	- now absurd (P).
-	- unfold dec.
-		now rewrite H1.
-Qed.
-
-Ltac case_dec a := let HDec := fresh in
-case_eq (# a); intro HDec;
-	[apply -> (dec_true a) in HDec | apply -> (dec_false a) in HDec].
-
-Lemma dec_ex : forall (P : Prop) `{Decidable P}, P \/ ~P.
-intros; case_dec P; auto.
-Qed.
-
-Lemma dec_notnot : forall (P : Prop) `{Decidable P}, ~~P  <-> P.
-split; [case_dec P |]; easy.
-Qed.
-
-Section not_dec.
-
-Variables (P : Prop) (d : Decidable P).
-Global Instance Not_dec : Decidable (~ P) := {}.
-{
-	case_dec P; tauto.
-}
+Lemma DecidableAsciiEq (a b : ascii) : (Decidable (a = b)).
+Proof.
+assert ({a = b} + {a <> b}) by repeat decide equality.
+destruct H; [ now left | now right ].
 Defined.
-End not_dec.
-
-Section logic_dec.
-
-Variables (A B : Prop) (dA : Decidable A) (dB : Decidable B).
-
-Global Instance And_dec : Decidable (A /\ B) := {}.
-{
-	case_dec A; [case_dec B |]; tauto.
-}
-Defined.
-
-Global Instance Or_dec : Decidable (A \/ B) := {}.
-{
-	case_dec A; [| case_dec B]; tauto.
-}
-Defined.
-
-Global Instance Im_dec : Decidable (A -> B) := {}.
-{
-	case_dec B; [| case_dec A]; tauto.
-}
-Defined.
-
-End logic_dec.
-
-Definition make_dec {P : Prop} (x : {P} + {~P}) : Decidable P := Build_Decidable P x.
-
-Section BoolDec.
-
-Variables (a b : bool).
-
-Global Instance DecidableBoolEq : (Decidable (a = b)) := {}.
-{
-	case a; case_eq b; intros; auto.
-	right; discriminate.
-}
-Defined.
-
-End BoolDec.
-
-Section AsciiDec.
-
-Variables (a b : ascii).
-
-Global Instance DecidableAsciiEq : (Decidable (a = b)) := {}.
-{
-	repeat decide equality.
-}
-Defined.
-
-End AsciiDec.
