fileSystem/theories/Spec/Props.v
@@ -8,22 +8,47 @@ Require Import String.
 Definition initialState := MkState (const None) (const None).
 
 Definition opened_fd (s : state) (fd : Z) : Prop :=
-	let (sfd, sfile) := s in
-	sfd fd <> None.
+	fds s fd <> None.
 Definition opened_file (s : state) (str : string) : Prop :=
-	let (sfd, sfile) := s in
-	exists (fd : Z), option_map file (sfd fd) = Some str.
+	exists (fd : Z), option_map file (fds s fd) = Some str.
+Definition opened_file_with_fd (s : state) (f : string) (fd : Z)
+	:= forall z, option_map file (fds s z) = Some f <-> fd = z.
 
-Definition fileContentKnown (s : fileState) : Prop
-	:= forall (n : N), content s n <> Unknownc.
+Lemma non_opened_fd_1 (s : state) (fd : Z) (file : string)
+	: ~ opened_fd s fd -> ~ opened_file_with_fd s file fd.
+Proof.
+intros H.
+unfold opened_file_with_fd.
+intro Hf.
+apply H.
+unfold opened_fd.
+intro Hf2.
+destruct (fds s fd) eqn:Heq.
++ discriminate Hf2.
++ pose (T := Hf fd).
+	replace (fds s fd) with (None (A:=fdState)) in T.
+	unfold option_map in T.
+	destruct T.
+	discriminate (H1 eq_refl).
+Qed.
 
-Definition sameFileContent (sStart sEnd : fileState) : Prop
-	:= fileContentKnown sStart
-		/\ forall (n : N), content sStart n = content sEnd n.
+Lemma opened_file_1 (s : state) (fd : Z) (file : string)
+	: opened_file_with_fd s file fd -> opened_file s file.
+Proof.
+edestruct 1.
+eexists.
+now apply H1.
+Qed.
 
-Definition sameFileContents (sStart sEnd : state) : Prop
-	:= forall (str : string) (sStartf : fileState), files sStart str = Some sStartf
-		-> exists (sEndf : fileState), files sEnd str = Some sEndf /\ sameFileContent sStartf sEndf.
+Definition fileContentKnown (f : string) (s : state) : Prop
+	:= match (files s f) with
+		| Some fs => forall (n : N), content fs n <> Unknownc
+		| None => False
+		end.
+
+Definition sameFileContent (f : string) (sStart sEnd : state) : Prop
+	:= fileContentKnown f sStart
+		/\ forall (n : N), option_map (fun x => content x n) (files sStart f) = option_map (fun x => content x n) (files sEnd f).
 
 Definition setFileContent (s : state) (str content : string) : state
 	:= let (sfd, sfile) := s in
@@ -35,3 +60,458 @@ Definition setFileContent (s : state) (str content : string) : state
 				)
 			) str in
 			MkState sfd sfile.
+
+Lemma fileContentKnownSetFileContent (file content : string) (s : state)
+	: fileContentKnown file (setFileContent s file content).
+Proof.
+unfold fileContentKnown.
+unfold setFileContent.
+destruct s.
+cbn.
+rewrite setFunOk.
+intros n.
+cbn.
+assert (forall m, addString content m (const Nonec) n <> Unknownc).
++ induction content.
+	- easy.
+	- intros m.
+		cbn.
+		admit.
+Admitted.
+
+Lemma setFileContent_fds (s : state) (str content : string) : fds s = fds (setFileContent s str content).
+Proof.
+now destruct s.
+Qed.
+
+Fixpoint setFileContents (s : state) (contents : list (string * string)) : state
+	:= match contents with
+	   | ((fn, fc)::contents)%list => setFileContents (setFileContent s fn fc) contents
+		 | _ => s
+		 end.
+
+Lemma setFileContents_fds (s : state) (contents : list (string * string))
+	: fds s = fds (setFileContents s contents).
+Proof.
+generalize s.
+induction contents; intros.
++ easy.
++ simpl.
+	destruct a.
+	rewrite <- IHcontents.
+	apply setFileContent_fds.
+Qed.
+
+Transparent abs_step.
+
+Section Abs_step_facts.
+
+Variable s : state.
+
+Lemma open_opened_fd (str : string) (fd : Z) (m : FileSystem.mode) (o : FileSystem.options)
+	: opened_fd (abs_step (FileSystem.Open m o str) fd s) fd.
+Proof.
+unfold opened_fd.
+destruct s.
+cbn.
+now rewrite setFunOk.
+Qed.
+
+Lemma open_opened_file_with_fd (str : string) (fd : Z) (m : FileSystem.mode) (o : FileSystem.options)
+	: ~ opened_file s str (* provable with the precondition *)
+		-> opened_file_with_fd (abs_step (FileSystem.Open m o str) fd s) str fd.
+Proof.
+unfold opened_file_with_fd.
+destruct s eqn:Heq.
+intros.
+constructor;
+	intros.
++ cbn in H0.
+	case_dec (fd = z).
+	- apply H1.
+	- rewrite setFunOk2 in H0.
+		* absurd (opened_file s str).
+			++ now subst.
+			++ exists z.
+				now subst.
+		* easy.
++	subst.
+	cbn.
+	now rewrite setFunOk.
+Qed.
+
+Lemma open_opened_file_with_fd2 (str f : string) (fd1 fd2 : Z) (m : FileSystem.mode) (o : FileSystem.options)
+	: opened_file_with_fd s f fd1
+		-> str <> f
+		-> opened_file_with_fd (abs_step (FileSystem.Open m o str) fd2 s) f fd1.
+Proof.
+unfold opened_file_with_fd.
+intros.
+destruct s.
+constructor;
+	intros.
++ apply H.
+	rewrite <- H1.
+	cbn.
+	case_dec (fd2 = z).
+	- subst.
+		rewrite setFunOk.
+		cbn.
+		destruct (fds z);
+			cbn.
+(*
+case_dec (fd2 = fd1).
++ subst.
+	intros.
+	exfalso.
+	eapply non_opened_fd_1 in H0.
+	apply H0.
+	apply H.
++ intros.
+	unfold opened_file_with_fd.
+	unfold opened_file_with_fd in H0.
+	destruct s eqn:Heq.
+	intros.
+	constructor;
+		intros.
+	-	case_dec (fd2 = z).
+		* subst.
+			cbn in H2.
+			rewrite setFunOk in H2.
+			cbn in H2.
+			cbn in H0.
+			inversion H2.
+			admit.
+		* apply H0.
+			cbn in H2.
+			now rewrite setFunOk2 in H2.
+	- subst.
+		cbn.
+		rewrite setFunOk2.
+		* now apply <- H0.
+		* apply H. *)
+Admitted.
+
+Lemma open_opened_fd2 (fd r : Z) (str : string) (m : FileSystem.mode) (o : FileSystem.options)
+	: opened_fd s fd -> opened_fd (abs_step (FileSystem.Open m o str) r s) fd.
+Proof.
+intros.
+unfold opened_fd.
+destruct s.
+cbn.
+case_dec (r = fd).
++ subst.
+	rewrite setFunOk.
+	unfold option_map.
+	now destruct (fds fd) eqn:Heq.
++ now rewrite setFunOk2.
+Qed.
+
+Lemma open_not_opened_file (r : Z) (str file : string) (m : FileSystem.mode) (o : FileSystem.options)
+	: ~ opened_file s file -> file <> str -> ~ opened_file (abs_step (FileSystem.Open m o str) r s) file.
+Proof.
+intros.
+destruct s.
+unfold opened_file.
+cbn.
+intro Hf.
+inversion Hf.
+clear Hf.
+case_dec (r = x).
++ subst.
+	rewrite setFunOk in H1.
+	cbn in H1.
+	inversion H1.
+	now subst.
++ rewrite setFunOk2 in H1.
+	- apply H.
+		now exists x.
+	- easy.
+Qed.
+
+Lemma getSize_opened_fd (fd1 fd2 : Z) (r : N)
+	: opened_fd s fd1 -> opened_fd (abs_step (FileSystem.GetSize fd2) r s) fd1.
+Proof.
+intros.
+now destruct s.
+Qed.
+
+Lemma getSize_not_opened_file (file : string) (fd : Z) (r : N)
+	: ~ opened_file s file -> ~ opened_file (abs_step (FileSystem.GetSize fd) r s) file.
+Proof.
+intros.
+destruct s.
+unfold opened_file.
+cbn.
+intro Hf.
+inversion Hf.
+apply H.
+unfold opened_file.
+cbn.
+now exists x.
+Qed.
+
+Lemma getSize_opened_file_with_fd (file : string) (fd1 fd2 : Z) (r : N)
+ : opened_file_with_fd s file fd1 -> opened_file_with_fd (abs_step (FileSystem.GetSize fd2) r s) file fd1.
+Proof.
+intros.
+now destruct s.
+Qed.
+
+Lemma read_opened_fd (n : N) (fd1 fd2 : Z) (r : string)
+	: opened_fd s fd1 -> opened_fd (abs_step (FileSystem.Read n fd2) r s) fd1.
+Proof.
+intros.
+unfold opened_fd.
+destruct s.
+cbn.
+case_dec (fd2 = fd1).
++ subst.
+	rewrite changeFunOk.
+	unfold option_map.
+	now destruct (fds fd1) eqn:Heq.
++ now rewrite changeFunOk2.
+Qed.
+
+Lemma read_not_opened_file (r file : string) (fd : Z) (n : N)
+	: ~ opened_file s file -> ~ opened_file (abs_step (FileSystem.Read n fd) r s) file.
+Proof.
+intros.
+destruct s.
+unfold opened_file.
+cbn.
+intro Hf.
+inversion Hf.
+apply H.
+unfold opened_file.
+cbn.
+exists x.
+rewrite <- H0.
+case_dec (fd = x).
++ subst.
+	rewrite changeFunOk.
+	unfold option_map.
+	destruct (fds x).
+	- now destruct f.
+	- reflexivity.
++ now rewrite changeFunOk2.
+Qed.
+
+Lemma read_opened_file_with_fd (file : string) (fd1 fd2 : Z) (n : N) (r : string)
+ : opened_file_with_fd s file fd1 -> opened_file_with_fd (abs_step (FileSystem.Read n fd2) r s) file fd1.
+Proof.
+intros.
+destruct s.
+unfold opened_file_with_fd.
+cbn.
+intros z.
+case_dec (fd2 = z).
++ subst.
+	split; intros.
+	- unfold opened_file_with_fd in H.
+		apply H.
+		rewrite <- H0.
+		rewrite changeFunOk.
+		cbn.
+		destruct (fds z).
+		* now destruct f.
+		* easy.
+	- subst.
+		rewrite changeFunOk.
+		unfold opened_file_with_fd in H.
+		pose (Hr := H z).
+		destruct Hr.
+		rewrite <- H1; try reflexivity.
+		cbn.
+		destruct (fds z).
+		* now destruct f.
+		* easy.
++ split; intros.
+	- unfold opened_file_with_fd in H.
+		apply H.
+		cbn.
+		rewrite <- H1.
+		now rewrite changeFunOk2.
+	- subst.
+		unfold opened_file_with_fd in H.
+		rewrite changeFunOk2.
+		* now apply <- H.
+		* assumption.
+Qed.
+
+Lemma write_opened_fd (str : string) (fd1 fd2 : Z) (r : unit)
+	: opened_fd s fd1 -> opened_fd (abs_step (FileSystem.Write str fd2) r s) fd1.
+Proof.
+intros.
+unfold opened_fd.
+destruct s.
+cbn.
+case_dec (fd2 = fd1).
++ subst.
+	rewrite changeFunOk.
+	unfold option_map.
+	now destruct (fds fd1) eqn:Heq.
++ now rewrite changeFunOk2.
+Qed.
+
+Lemma write_opened_file (str file : string) (fd : Z) (r : unit)
+	: opened_file s file -> opened_file (abs_step (FileSystem.Write str fd) r s) file.
+Proof.
+intros.
+destruct s.
+unfold opened_file.
+cbn.
+inversion H.
+exists x.
+rewrite <- H0.
+case_dec (fd = x).
++ subst.
+	rewrite changeFunOk.
+	unfold option_map.
+	cbn.
+	destruct (fds x).
+	- now destruct f.
+	- reflexivity.
++ now rewrite changeFunOk2.
+Qed.
+
+Lemma write_not_opened_file (str file : string) (fd : Z) (r : unit)
+	: ~ opened_file s file -> ~ opened_file (abs_step (FileSystem.Write str fd) r s) file.
+Proof.
+intros.
+destruct s.
+unfold opened_file.
+cbn.
+intro Hf.
+inversion Hf.
+apply H.
+unfold opened_file.
+cbn.
+exists x.
+rewrite <- H0.
+case_dec (fd = x).
++ subst.
+	rewrite changeFunOk.
+	unfold option_map.
+	destruct (fds x).
+	- now destruct f.
+	- reflexivity.
++ now rewrite changeFunOk2.
+Qed.
+
+Lemma write_opened_file_with_fd (file : string) (fd1 fd2 : Z) (r : unit) (str : string)
+ : opened_file_with_fd s file fd1 -> opened_file_with_fd (abs_step (FileSystem.Write str fd2) r s) file fd1.
+Proof.
+intros.
+destruct s.
+unfold opened_file_with_fd.
+cbn.
+intros z.
+case_dec (fd2 = z).
++ subst.
+	split; intros.
+	- unfold opened_file_with_fd in H.
+		apply H.
+		rewrite <- H0.
+		rewrite changeFunOk.
+		cbn.
+		destruct (fds z).
+		* now destruct f.
+		* easy.
+	- subst.
+		rewrite changeFunOk.
+		unfold opened_file_with_fd in H.
+		pose (Hr := H z).
+		destruct Hr.
+		rewrite <- H1; try reflexivity.
+		cbn.
+		destruct (fds z).
+		* now destruct f.
+		* easy.
++ split; intros.
+	- unfold opened_file_with_fd in H.
+		apply H.
+		cbn.
+		rewrite <- H1.
+		now rewrite changeFunOk2.
+	- subst.
+		unfold opened_file_with_fd in H.
+		rewrite changeFunOk2.
+		* now apply <- H.
+		* assumption.
+Qed.
+
+Lemma close_opened_fd (fd1 fd2 : Z) (r : unit)
+	: opened_fd s fd1 -> fd2 <> fd1 -> opened_fd (abs_step (FileSystem.Close fd2) r s) fd1.
+Proof.
+intros.
+unfold opened_fd.
+destruct s.
+cbn.
+now rewrite setFunOk2.
+Qed.
+
+Lemma close_not_opened_file (f : string) (fd : Z) (r : unit)
+	: ~ opened_file s f -> ~ opened_file (abs_step (FileSystem.Close fd) r s) f.
+Proof.
+intros.
+destruct s.
+unfold opened_file.
+cbn.
+intro Hf.
+inversion Hf.
+case_dec (fd = x).
++ subst.
+	now rewrite setFunOk in H0.
++ rewrite setFunOk2 in H0.
+	- apply H.
+		now exists x.
+	- easy.
+Qed. 
+
+Lemma close_not_opened_file2 (f : string) (fd : Z) (r : unit)
+	: opened_file_with_fd s f fd
+		-> ~ opened_file (abs_step (FileSystem.Close fd) r s) f.
+Proof.
+intros.
+destruct s.
+unfold opened_file.
+cbn.
+unfold opened_file_with_fd in H.
+intro Hf.
+inversion Hf.
+clear Hf.
+case_dec (fd = x).
++ subst.
+	now rewrite setFunOk in H0.
++ apply H1.
+	apply (H x).
+	now rewrite setFunOk2 in H0.
+Qed.
+
+Lemma close_opened_file_with_fd (f : string) (fd1 fd2 : Z) (r : unit)
+	: opened_file_with_fd s f fd1
+		-> fd1 <> fd2 (* provable with the postcondition of the corresponding open *)
+		-> opened_file_with_fd (abs_step (FileSystem.Close fd2) r s) f fd1.
+Proof.
+intros.
+destruct s.
+unfold opened_file_with_fd.
+Admitted.
+
+Lemma unlink_not_opened_file (file z : string) (r : unit)
+	: ~ opened_file s file -> ~ opened_file (abs_step (FileSystem.Unlink z) r s) file.
+Proof.
+intros.
+destruct s.
+unfold opened_file.
+cbn.
+intro Hf.
+inversion Hf.
+apply H.
+unfold opened_file.
+cbn.
+now exists x.
+Qed.
+
+End Abs_step_facts.
