fileSystem/theories/Spec/State.v
@@ -45,6 +45,14 @@ destruct (H i).
 now destruct is_dec.
 Qed.
 
+Lemma setFunOk2 {A B} (f : A -> B) (n : B) (i j : A) `{forall (b : A), Decidable (i = b)}
+	: i <> j -> setFun f n i j = f j.
+Proof.
+compute.
+destruct (H j).
+now destruct is_dec.
+Qed.
+
 Definition changeFun {A B} (f : A -> B) (fn : B -> B) (i : A) `{forall (b : A), Decidable (i = b)} : A -> B :=
 fun (j : A) => if (# (i = j)) then fn (f j) else f j.
 
@@ -56,23 +64,113 @@ destruct (H i).
 now destruct is_dec.
 Qed.
 
+Lemma changeFunOk2 {A B} (f : A -> B) (fn : B -> B) (i j : A) `{forall (b : A), Decidable (i = b)}
+	: i <> j -> changeFun f fn i j = f j.
+Proof.
+compute.
+destruct (H j).
+now destruct is_dec.
+Qed.
+
 Fixpoint addString (s : string) (p : N) (c : funString) : funString :=
 	match s with
 	| String n ns => addString ns (p + 1) (setFun c (Somec n) p)
 	| _ => c
 	end.
 
-Fixpoint getString_aux (n : nat) (p : N) (c : funString) (acc : string) : option string :=
+Lemma addStringOk1 (s : string) (n p : N) (c : funString)
+	: (n < p)%N -> addString s p c n = c n.
+Proof.
+revert p c n.
+induction s.
++ easy.
++ intros.
+	cbn.
+	rewrite IHs.
+	- rewrite setFunOk2.
+		* reflexivity.
+		* lia.
+	- lia.
+Qed.
+
+Lemma addStringOk2 (s : string) (n p : N) (c : funString)
+	: (n >= p)%N -> (n < p + (N.of_nat (length s)))%N -> Some (addString s p c n) = option_map Somec (get (N.to_nat (n - p)%N) s).
+Proof.
+destruct s.
++ intros.
+	cbn in H0.
+	lia.
++ revert p c n a.
+	induction s.
+	- intros.
+		cbn.
+		destruct (n - p)%N eqn:Heq.
+		* assert (n = p) by lia.
+			subst.
+			now rewrite setFunOk.
+		* cbn in H0.
+			lia.
+	- intros.
+		change (addString (String a0 (String a s)) p c n) with (addString (String a s) (p + 1) (setFun c (Somec a0) p) n).
+		rewrite IHs.
+		* cbn.
+			f_equal.
+			pose (m := (N.to_nat (n - (p + 1)))).
+			fold m.
+			replace (N.to_nat (n - p)) with (S m).
+			++ destruct m; reflexivity.
+			++ unfold m.
+				rewrite <- Nnat.N2Nat.inj_succ.
+				f_equal.
+				admit.
+		* cbn in H0.
+			admit.
+		* cbn in H0.
+			cbn.
+			lia.
+Admitted.
+
+Lemma addStringOk3 (s : string) (n p : N) (c : funString)
+	: (n >= p + (N.of_nat (length s)))%N -> addString s p c n = c n.
+Proof.
+revert p c n.
+induction s.
++ easy.
++ intros.
+	cbn.
+	rewrite IHs.
+	- rewrite setFunOk2.
+		* reflexivity.
+		* cbn in H.
+			lia.
+	- cbn in H.
+		lia.
+Qed.
+
+Fixpoint getString_aux (n : nat) (p : N) (c : funString) : option string :=
 	match n with
 	| S m => match c p with
-		|	Somec ch => getString_aux m (p + 1) c (acc ++ String ch "")
+		|	Somec ch => option_map (String ch) (getString_aux m (p + 1) c)
 		|	_ => None
 		end
-	| _ => Some acc
+	| _ => Some ""%string
 	end.
 
 Definition getString (n : N) (p : N) (c : funString) : option string :=
-	getString_aux (N.to_nat n) p c "".
+	getString_aux (N.to_nat n) p c.
+
+Lemma getAddString (s : string) (p : N) (c : funString)
+	: getString (N.of_nat (length s)) p (addString s p c) = Some s.
+Proof.
+revert p c.
+induction s.
++ easy.
++ intros p c.
+	cbn.
+	rewrite SuccNat2Pos.id_succ.
+	unfold getString in IHs.
+	rewrite Nnat.Nat2N.id in IHs.
+Admitted.
 
 Definition setFile (f : string -> string) (s : fdState) :=
 	let (a, b, c) := s in MkFdState (f a) b c.
@@ -85,77 +183,3 @@ Definition setSize (f : option N -> option N) (s : fileState) :=
 	let (a, b) := s in MkFileState (f a) b.
 Definition setContent (f : funString -> funString) (s : fileState) :=
 	let (a, b) := s in MkFileState a (f b).
-
-(*
------
-
-Definition partial (A B : Type) := A -> option B.
-
-Definition setFun {A B} (f : A -> B) (n : B) (i : A) `{forall (b : A), Decidable (i = b)} : A -> B :=
-fun (j : A) => if (# (i = j)) then n else f j.
-
-Lemma setFunOk {A B} (f : A -> B) (n : B) (i : A) `{forall (b : A), Decidable (i = b)}
-	: setFun f n i i = n.
-Proof.
-compute.
-destruct (H i).
-now destruct is_dec.
-Qed.
-
-Definition changeFun {A B} (f : A -> B) (fn : B -> B) (i : A) `{forall (b : A), Decidable (i = b)} : A -> B :=
-fun (j : A) => if (# (i = j)) then fn (f j) else f j.
-
-Lemma changeFunOk {A B} (f : A -> B) (fn : B -> B) (i : A) `{forall (b : A), Decidable (i = b)}
-	: changeFun f fn i i = fn (f i).
-Proof.
-compute.
-destruct (H i).
-now destruct is_dec.
-Qed.
-
-(* Compute (setFun (fun a : nat => a + 1) 5 3 1). *) (* -> Anomaly without decidableNatEq *)
-
-Definition fdContent := partial Z ascii.
-
-Fixpoint addString (s : string) (p : N) (c : fdContent) : fdContent :=
-	match s with
-	| String n ns => addString ns (p + 1) (setFun c (Some n) (Z.of_N p))
-	| _ => c
-	end.
-
-Fixpoint getString_aux (n : nat) (p : N) (c : fdContent) (acc : string) : option string :=
-	match n with
-	| S m => match c (Z.of_N p) with
-		|	Some ch => getString_aux m (p + 1) c (acc ++ String ch "")
-		|	_ => None
-		end
-	| _ => Some acc
-	end.
-
-Definition getString (n : N) (p : N) (c : fdContent) : option string :=
-	getString_aux (N.to_nat n) p c "".
-
-Record fdState : Type := MkFdState
-{
-	mode : FileSystem.mode;
-	kind : option FileSystem.fileKind;
-	size : option N;
-	pos : option N;
-	content : fdContent;
-}.
-
-Definition setMode (f : FileSystem.mode -> FileSystem.mode) (s : fdState) :=
-	let (a, b, c, d, e) := s in MkFdState (f a) b c d e.
-Definition setKind
-	(f : option FileSystem.fileKind -> option FileSystem.fileKind) (s : fdState) :=
-	let (a, b, c, d, e) := s in MkFdState a (f b) c d e.
-Definition setSize (f : option N -> option N) (s : fdState) :=
-	let (a, b, c, d, e) := s in MkFdState a b (f c) d e.
-Definition setPos (f : option N -> option N) (s : fdState) :=
-	let (a, b, c, d, e) := s in MkFdState a b c (f d) e.
-Definition setContent (f : fdContent -> fdContent) (s : fdState) :=
-	let (a, b, c, d, e) := s in MkFdState a b c d (f e).
-
-Definition state := partial Z fdState.
-
-*)
