ar/theories/Proof.v
@@ -1,0 +1,648 @@
+Require Import FreeSpec.Stdlib.FileSystem.Definitions.
+Require Import FreeSpec.Stdlib.FileSystem.Specifications.
+Require Import FreeSpec.Stdlib.FileSystem.Spec.Props.
+Require Import FreeSpec.Tactics.
+Require Import FreeSpec.Interface.
+Require Import FreeSpec.Program.
+Require Import FreeSpec.Semantics.
+Require Import FreeSpec.Specification.
+Require Import Coq.Program.Equality.
+From Equations Require Import Equations.
+Require Import Prelude.Control.
+Require Import String.
+Require Import ArMain.
+Require Import BinInt.
+Require Import BinNat.
+Require Import List.
+Require Import Util.Util.
+
+Local Open Scope prelude_scope.
+
+Ltac inversion_subst H :=
+	inversion H; 
+	clear H;
+	repeat (simpl_existTs; subst).
+
+(* Definition remove_files {ix} `{Use FileSystem.i ix} (files : list string)
+	: Program ix unit := fold_left (fun p file => p ;; FileSystem.unlink file) files (pure tt). *)
+
+Fixpoint remove_files {ix} `{Use FileSystem.i ix} (files : list string)
+	: Program ix unit :=
+	match files with
+	| nil => pure tt
+	| file :: files => FileSystem.unlink file ;; remove_files files
+	end.
+
+Definition ar_id {ix} `{Use FileSystem.i ix} (files : list string) (ar : string)
+	: Program ix unit :=
+	Ar.create files ar;;
+	remove_files files;;
+	Ar.extract ar;;
+	pure tt.
+
+Section Proof.
+
+(* write_header proofs *)
+
+Lemma write_header_spec (fd : Z) (s : state)
+	: opened_fd s fd -> write_header fd |> specs[s].
+Proof.
+intros.
+constructor.
++ constructor.
+	apply H.
++ constructor.
+Qed.
+
+Lemma correct_write_header_1 (fd : Z) (r : unit) (w w' : state)
+	: correct_run specs w (write_header fd) r w' -> opened_fd w' fd.
+Proof.
+intros.
+inversion_subst H.
+inversion_subst Hop.
+inversion_subst Hf.
+now apply write_opened_fd.
+Qed.
+
+Lemma correct_write_header_2 (fd z : Z) (r : unit) (w w' : state)
+	: opened_fd w fd -> correct_run specs w (write_header z) r w' -> opened_fd w' fd.
+Proof.
+intros.
+inversion_subst H0.
+inversion_subst Hf.
+now apply write_opened_fd.
+Qed.
+
+Lemma correct_write_header_3 (z : Z) (f : string) (r : unit) (w w' : state)
+	: ~ opened_file w f -> correct_run specs w (write_header z) r w'
+		-> ~ opened_file w' f.
+Proof.
+intros.
+inversion_subst H0.
+inversion_subst Hf.
+now apply write_not_opened_file.
+Qed.
+
+Lemma correct_write_header_4 (fd : Z) (file : string) (r : unit) (w w' : state)
+	: opened_file_with_fd w file fd -> correct_run specs w (write_header fd) r w'
+		-> opened_file_with_fd w' file fd.
+Proof.
+intros.
+inversion_subst H0.
+inversion_subst Hf.
+now apply write_opened_file_with_fd.
+Qed.
+Opaque write_header.
+
+(* write_entry proofs *)
+
+Lemma write_entry_spec (fd : Z) (name : string) (s : state)
+	: ~ opened_file s name -> opened_fd s fd -> write_entry fd name |> specs[s].
+Proof.
+constructor.
++ constructor.
+	apply H.
++ constructor.
+	- constructor.
+		apply open_opened_fd.
+	- constructor.
+		* constructor.
+			apply getSize_opened_fd.
+			apply open_opened_fd.
+		* constructor.
+			++ constructor.
+				apply read_opened_fd.
+				apply getSize_opened_fd.
+				apply open_opened_fd.
+			++ assert (x <> fd).
+				-- inversion_subst Hpost.
+					intro Hf.
+					now subst.
+				-- constructor.
+					** constructor.
+						apply close_opened_fd.
+						+++ apply read_opened_fd.
+							apply getSize_opened_fd.
+							now apply open_opened_fd2.
+						+++ apply H1.
+						** constructor.
+							+++ constructor.
+								apply write_opened_fd.
+								apply close_opened_fd.
+								--- apply read_opened_fd.
+									apply getSize_opened_fd.
+									now apply open_opened_fd2.
+								--- apply H1.
+							+++ constructor.
+								--- constructor.
+									apply write_opened_fd.
+									apply write_opened_fd.
+									apply close_opened_fd.
+									*** apply read_opened_fd.
+										apply getSize_opened_fd.
+										now apply open_opened_fd2.
+									*** apply H1.
+								--- constructor.
+Qed.
+
+Lemma correct_write_entry_1 (fd z : Z) (name : string) (r : unit) (w w' : state)
+	: opened_fd w fd -> correct_run specs w (write_entry z name) r w'
+		-> opened_fd w' fd.
+Proof.
+intros.
+inversion_subst H0.
+inversion_subst Hf.
+inversion_subst Hf0.
+inversion_subst Hf.
+inversion_subst Hf0.
+inversion_subst Hf.
+inversion_subst Hf0.
+inversion_subst Hf.
+assert (Hxfd : x <> fd).
++ inversion_subst Hx.
+	intro Hf.
+	now subst.
++ apply write_opened_fd.
+	apply write_opened_fd.
+	apply write_opened_fd.
+	apply close_opened_fd.
+	- apply read_opened_fd.
+		apply getSize_opened_fd.
+		now apply open_opened_fd2.
+	- apply Hxfd.
+Qed.
+
+Lemma correct_write_entry_2_aux (f : string) (z : Z) (name : string) (r : unit) (w w' : state)
+	: ~ opened_file w f -> correct_run specs w (write_entry z name) r w'
+		-> ~ opened_file w' f.
+Proof.
+intros.
+inversion_subst H0.
+inversion_subst Hf.
+inversion_subst Hf0.
+inversion_subst Hf.
+inversion_subst Hf0.
+inversion_subst Hf.
+inversion_subst Hf0.
+inversion_subst Hf.
+apply write_not_opened_file.
+apply write_not_opened_file.
+apply write_not_opened_file.
+case_dec (f = name).
++ subst.
+	apply close_not_opened_file2.
+	- apply read_opened_file_with_fd.
+		apply getSize_opened_file_with_fd.
+		now apply open_opened_file_with_fd.
++ apply close_not_opened_file.
+	apply read_not_opened_file.
+	apply getSize_not_opened_file.
+	now apply open_not_opened_file.
+Qed.
+
+Lemma correct_write_entry_2 (fs : list string) (z : Z) (name : string) (r : unit) (w w' : state)
+	: Forall (fun f => ~ opened_file w f) fs
+		-> correct_run specs w (write_entry z name) r w'
+		-> Forall (fun f => ~ opened_file w' f) fs.
+Proof.
+intros.
+induction H.
++ constructor.
++ constructor.
+	- now apply (correct_write_entry_2_aux x z name r w).
+	- apply IHForall.
+Qed.
+
+Lemma correct_write_entry_3 (f file : string) (fd : Z) (r : unit) (w w' : state)
+	: opened_file_with_fd w file fd
+		-> correct_run specs w (write_entry fd f) r w'
+		-> opened_file_with_fd w' file fd.
+Proof.
+intros.
+inversion_subst H0.
+inversion_subst Hf.
+inversion_subst Hf0.
+inversion_subst Hf.
+inversion_subst Hf0.
+inversion_subst Hf.
+inversion_subst Hf0.
+inversion_subst Hf.
+apply write_opened_file_with_fd.
+apply write_opened_file_with_fd.
+apply write_opened_file_with_fd.
+case_dec (fd = x).
++ subst.
+	inversion_subst Hx.
+	exfalso.
+	apply (non_opened_fd_1 _ _ _ H5 H).
++ apply close_opened_file_with_fd.
+	- apply read_opened_file_with_fd.
+		apply getSize_opened_file_with_fd.
+		apply open_opened_file_with_fd2.
+		* apply H.
+		* intro Hf.
+			subst.
+			inversion_subst Hop.
+			apply Hno.
+			now eapply opened_file_1.
+	- apply H0.
+Qed.
+
+Lemma correct_write_entry_4 (fd : Z) (name : string) (r : unit) (w w' : state)
+	: correct_run specs w (write_entry fd name) r w'
+		-> True. (* The file name is written. *)
+Proof.
+Admitted.
+Opaque write_entry.
+
+(* create_aux_rec proofs *)
+
+Lemma create_aux_rec_spec (fn : list string) (fd : Z) (s : state)
+	: Forall (fun fn => ~ opened_file s fn) fn
+		-> opened_fd s fd
+		-> create_aux_rec fd fn |> specs[s].
+Proof.
+revert s.
+induction fn.
++ constructor.
++ cbn.
+	intros.
+	apply correct_program_correct_run_correct_bind.
+	- apply write_entry_spec.
+		* now inversion H.
+		* apply H0.
+	- intros.
+		apply IHfn.
+		* inversion H.
+			subst.
+			eapply correct_write_entry_2.
+			++ apply H5.
+			++ apply H1.
+		* eapply correct_write_entry_1.
+			++ apply H0.
+			++ apply H1.
+Qed.
+
+Lemma correct_create_aux_rec_1 (fn : list string) (fd : Z) (r : unit) (w w' : state)
+	: opened_fd w fd
+		-> correct_run specs w (create_aux_rec fd fn) r w' -> opened_fd w' fd.
+Proof.
+intros.
+revert w H H0.
+induction fn.
++ intros.
+	now inversion_subst H0.
++ intros.
+	cbn in H0.
+	apply correct_run_program_bind in H0.
+	inversion_subst H0.
+	inversion_subst H1.
+	destruct H0.
+	apply (IHfn x0).
+	- eapply correct_write_entry_1.
+		* apply H.
+		* apply H0.
+	- apply H1.
+Qed.
+
+Lemma correct_create_aux_rec_2 (fn : list string) (file : string) (fd : Z) (r : unit) (w w' : state)
+	: ~ opened_file w file
+		-> correct_run specs w (create_aux_rec fd fn) r w'
+		-> ~ opened_file w' file.
+Proof.
+intros.
+revert w H H0.
+induction fn.
++ intros.
+	now inversion_subst H0.
++ intros.
+	cbn in H0.
+	apply correct_run_program_bind in H0.
+	inversion_subst H0.
+	inversion_subst H1.
+	destruct H0.
+	apply (IHfn x0).
+	- eapply correct_write_entry_2_aux.
+		* apply H.
+		* apply H0.
+	- apply H1.
+Qed.
+
+Lemma correct_create_aux_rec_3 (fn : list string) (file : string) (fd : Z) (r : unit) (w w' : state)
+	: opened_file_with_fd w file fd
+		-> correct_run specs w (create_aux_rec fd fn) r w'
+		-> opened_file_with_fd w' file fd.
+Proof.
+intros.
+revert w H H0.
+induction fn.
++ intros.
+	now inversion_subst H0.
++ intros.
+	cbn in H0.
+	apply correct_run_program_bind in H0.
+	inversion_subst H0.
+	inversion_subst H1.
+	destruct H0.
+	apply (IHfn x0).
+	- eapply correct_write_entry_3.
+		* apply H.
+		* apply H0.
+	- apply H1.
+Qed.
+
+Opaque create_aux_rec.
+
+(* create_aux (Ar.create) proofs *)
+
+Lemma ar_create_spec (fn : list string) (output : string) (s : state)
+	: ~ In output fn -> (forall f, ~ opened_file s f)
+		-> Ar.create fn output |> specs[s].
+Proof.
+intros.
+prove_program.
++ constructor.
+	apply H0.
++ apply write_header_spec.
+	apply open_opened_fd.
++ apply create_aux_rec_spec.
+	- apply Forall_forall.
+		intros.
+		eapply correct_write_header_3;
+			revgoals.
+		* apply Hrun.
+		* apply open_not_opened_file.
+			++ apply (H0 x0).
+			++ intro Hf.
+				now subst.
+	- eapply correct_write_header_1.
+		apply Hrun.
++ constructor.
+	eapply correct_create_aux_rec_1;
+		revgoals.
+	- apply Hrun0.
+	- eapply correct_write_header_1.
+		apply Hrun.
+Qed.
+
+Lemma correct_ar_create (fn : list string) (output : string) (r : bool) (w1 w2 : state) (file : string)
+	: (forall f : string, ~ opened_file w1 f)
+	-> correct_run specs w1 (Ar.create fn output) r w2
+	-> ~ opened_file w2 file.
+Proof.
+intro Hout.
+intros.
+cbn in H.
+inversion_subst H.
+apply correct_run_program_bind in Hf.
+inversion_subst Hf.
+inversion_subst H.
+destruct H0.
+apply correct_run_program_bind in H.
+inversion_subst H.
+inversion_subst H1.
+destruct H.
+inversion_subst H0.
+apply correct_run_program_bind in H1.
+inversion_subst H1.
+inversion_subst H0.
+destruct H1.
+inversion_subst H1.
+inversion_subst Hf.
+case_dec (file = output).
++ subst.
+	apply close_not_opened_file2.
+	eapply correct_create_aux_rec_3.
+	- eapply correct_write_header_4;
+			revgoals.
+		* apply H.
+		* apply open_opened_file_with_fd.
+			apply Hout.
+	- apply H0.
++ apply close_not_opened_file.
+	eapply correct_create_aux_rec_2.
+	- eapply correct_write_header_3;
+			revgoals.
+		* apply H.
+		* apply open_not_opened_file.
+			++ apply Hout.
+			++ apply H1.
+	- apply H0.
+Qed.
+Opaque Ar.create.
+
+(* remove_files proofs *)
+
+Lemma remove_files_spec (fn : list string) (s : state)
+	: remove_files fn |> specs[s].
+Proof.
+revert s.
+induction fn.
++ constructor.
++ cbn.
+	constructor.
+	- constructor.
+	- intros.
+		apply IHfn.
+Qed.
+
+(* Transparent abs_step.
+Lemma correct_remove_files (r : unit) (w0 w1 : state)
+	: correct_run specs w0 (remove_files file_names) r w1
+		-> fds w0 = fds w1.
+Proof.
+intros.
+destruct w0 as [fds0 files0].
+destruct w1 as [fds1 files1].
+cbn.
+revert fds0 files0 fds1 files1 H.
+induction file_names; intros.
++ now inversion H.
++ cbn in H.
+	inversion_subst H.
+	cbn in Hf.
+	eapply IHl.
+	apply Hf.
+Qed.
+Opaque abs_step. *)
+
+Lemma correct_remove_files (fn : list string) (r : unit) (w0 w1 : state) (file : string)
+	: ~ opened_file w0 file
+		-> correct_run specs w0 (remove_files fn) r w1
+		-> ~ opened_file w1 file.
+Proof.
+intros.
+revert w0 H H0.
+induction fn;
+	intros.
++ now inversion_subst H0.
++ cbn in H0.
+	inversion_subst H0.
+	cbn in Hf.
+	eapply IHfn;
+		revgoals.
+	- apply Hf.
+	- apply unlink_not_opened_file.
+		apply H.
+Qed.
+Opaque remove_files.
+
+(* read_entry proofs *) 
+
+Lemma read_entry_spec (output : string) (h : string) (fd : Z) (s : state)
+	: (forall (file : string), file <> output -> ~ opened_file s file)
+		-> opened_fd s fd
+		-> read_entry h fd |> specs[s].
+Proof.
+intros.
+prove_program.
++ constructor.
+	apply H0.
++ constructor.
+	apply read_not_opened_file.
+	apply H.
+	intro Hf.
+
+	admit. (* input <> output *)
++ constructor.
+	apply open_opened_fd.
++ constructor.
+	apply write_opened_fd.
+	apply open_opened_fd.
+Admitted.
+
+Lemma correct_read_entry (h : string) (fd : Z) (w0 w1 : state) (r : N)
+	: correct_run specs w0 (read_entry h fd) r w1 -> True.
+Proof.
+auto.
+Qed.
+Opaque read_entry.
+
+(* extract_aux_rec proofs *)
+
+Lemma extract_aux_rec_spec (output : string) (fd : Z) (size : N) (s : state)
+	: (forall (file : string), file <> output -> ~ opened_file s file)
+		-> opened_fd s fd -> extract_aux_rec fd size |> specs[s].
+Proof.
+intros.
+funelim (extract_aux_rec fd size).
++ constructor.
++ constructor.
+	- constructor.
+		apply H2.
+	- intros.
+		destruct x.
+		* constructor.
+		* apply correct_program_correct_run_correct_bind.
+			++ eapply read_entry_spec.
+				-- intros.
+					apply read_not_opened_file.
+					apply H1.
+					apply H.
+				-- apply read_opened_fd.
+					apply H2.
+			++ intros.
+				admit. (* Induction avec Equations *)
+Admitted.
+
+Lemma correct_extract_aux_rec (fd : Z) (size : N) (w0 w1 : state) (r : unit)
+	: opened_fd w0 fd
+		-> correct_run specs w0 (extract_aux_rec fd size) r w1
+		-> opened_fd w1 fd.
+Proof.
+intros.
+funelim (extract_aux_rec fd size).
++ rewrite <- Heqcall in H1.
+	now inversion_subst H1.
++ rewrite <- Heqcall in H2.
+	inversion_subst H2.
+	inversion_subst Hf.
+	- now apply read_opened_fd.
+	- admit. (* Induction avec Equations *)
+Admitted.
+Opaque extract_aux_rec.
+
+(* extract_aux (Ar.extract) proofs *)
+
+Lemma ar_extract_spec (output : string) (s : state)
+	: (forall f, ~ opened_file s f)
+		-> Ar.extract output |> specs[s].
+Proof.
+intros.
+prove_program.
++ constructor.
+	apply H.
++ constructor.
+	apply open_opened_fd.
++ eapply extract_aux_rec_spec.
+	- intros.
+		apply getSize_not_opened_file.
+		apply open_not_opened_file.
+		* apply H.
+		* apply H0.
+	- apply getSize_opened_fd.
+		apply open_opened_fd.
++ constructor.
+	eapply correct_extract_aux_rec;
+		revgoals.
+	- apply Hrun.
+	- apply getSize_opened_fd.
+		apply open_opened_fd.
+Qed.
+Opaque Ar.extract.
+
+(* This list contains the input: each pair contains a file name and its
+	supposed content *)
+Variable input : list (string * string).
+
+Definition file_names := map fst input.
+Definition file_contents := map snd input.
+
+(* This string is the produced ar name. It must not be in file_names *)
+Variable output : string.
+
+(* The initial state : empty state with each file content added *)
+Definition initial_state := setFileContents initialState input.
+
+Definition prog := ar_id file_names output.
+
+Lemma initial_not_opened (str : string) : ~ (opened_file initial_state str).
+Proof.
+unfold opened_file.
+rewrite <- setFileContents_fds.
+now inversion 1.
+Qed.
+
+(* The program fulfill the specification of the interface *)
+
+(* Hypothesis : the output file is not in the input list *)
+(*              all input files names are not too long *)
+Parameter output_not_in_input : ~(In output file_names).
+Parameter input_files_names_length : Forall (fun name => String.length name <= 15) file_names.
+
+Theorem ar_spec : ar_id file_names output |> specs[initial_state].
+Proof.
+prove_program.
++ apply ar_create_spec.
+	- apply output_not_in_input.
+	- intros.
+		apply initial_not_opened.
++ apply remove_files_spec.
++ apply ar_extract_spec.
+	intro f.
+	eapply correct_remove_files;
+		revgoals.
+	- apply Hrun0.
+	- eapply correct_ar_create.
+		* apply initial_not_opened.
+		* apply Hrun.
+Qed.
+
+Theorem ar_correct (final_state : state) (r : unit)
+	: correct_run specs initial_state (ar_id file_names output) r final_state
+	-> Forall (fun f => sameFileContent f initial_state final_state) file_names.
+Proof.
+admit.
+Admitted.
+
+End Proof.
