fileSystem/demos/Cat.v
@@ -19,14 +19,14 @@
  *)
 
 Require Import FreeSpec.Stdlib.Console.
-Require Import FreeSpec.Stdlib.FileSystem.
+Require Import FreeSpec.Stdlib.FileSystem.Definitions.
 Require Import FreeSpec.Program.
 Require Import Prelude.Control.
 
 Local Open Scope prelude_scope.
 
 Definition cat {ix} `{Use Console.i ix} `{Use FileSystem.i ix} : Program ix unit :=
-  fd <- FileSystem.open FileSystem.ReadOnly FileSystem.N "Cat.v";
+  fd <- FileSystem.open FileSystem.ReadOnly FileSystem.DontCreate "Cat.v";
   size <- FileSystem.getSize fd;
   FileSystem.read size fd >>= Console.echo;;
   FileSystem.close fd.
