fileSystem/theories/Specifications.v
@@ -1,0 +1,4 @@
+Require Export Spec.State.
+Require Export Spec.Props.
+Require Export Spec.Spec.
+Require Export Spec.Step.
