util/theories/Util.v
@@ -1,0 +1,49 @@
+Require Import BinNat.
+Require Import Lia.
+From Equations Require Import Equations.
+
+(* Needed to use wf recursion on type N *)
+Global Instance lt_wf : WellFounded N.lt.
+Proof.
+intro x.
+induction x using N.peano_ind.
++ constructor.
+	intros y Hy.
+	lia.
++ constructor.
+	intros y Hy. 
+	apply N.lt_succ_r in Hy.
+	apply N.le_lteq in Hy.
+	destruct Hy.
+	- constructor.
+		inversion IHx.
+		now apply H0.
+	- now subst.
+Qed.
+
+Require Import FreeSpec.Program.
+Require Import FreeSpec.Specification.
+
+Lemma correct_run_program_bind
+      {I:         Type -> Type}
+      {A B W:     Type}
+      (c:         Specification W I)
+      (w w':      W)
+      (p:         Program I A)
+      (f:         A -> Program I B)
+      (x:         B)
+  : correct_run c w (program_bind p f) x w'
+		-> exists y w'', correct_run c w p y w''
+			/\ correct_run c w'' (f y) x w'.
+Proof.
+intros.
+revert B f x H.
+induction p.
++ exists a.
+       exists w.
+       constructor.
+       - constructor.
+       - now cbn in H.
++	admit.
+Admitted.
+
